Bloom filter passes verification (although with some assumptions)

examples/crypto/bloom.fst
@@ -34,7 +34,7 @@ type hash_fn = text -> Tot hash
 type bloom (ln:ln_t) = bl:seq bool{Seq.length bl = ln}
 
 (* TODO: put this as an anonymous function in le *)
-val le_loop: ln:ln_t -> i:uint16{i<=ln} -> bl1: bloom ln -> bl2: bloom ln -> Tot bool
+val le_loop: ln:ln_t -> i:uint16{i <= ln} -> bl1: bloom ln -> bl2: bloom ln -> Tot bool (decreases %[ln - i])
 let rec le_loop ln i bl1 bl2 =
   if i < ln then
   begin
@@ -48,10 +48,25 @@ let rec le_loop ln i bl1 bl2 =
 val le: ln:ln_t -> bl1:bloom ln -> bl2:bloom ln -> Tot bool
 let le ln bl1 bl2 = le_loop ln 0 bl1 bl2
 
+assume val lemma_le_eq: ln:ln_t -> bl:bloom ln -> Lemma
+  (requires True)
+  (ensures (le ln bl bl))
+
+(*val set: ln:ln_t -> bl:bloom ln -> i:uint16 -> Tot (bl':bloom ln{le ln bl bl'})
+let set ln bl i =
+  let i' = op_Modulus i ln in
+  let bl' = Seq.upd bl i' true in
+  assert ((not (Seq.index bl i')) || (Seq.index bl' i'));
+  bl'*)
+
 val set: ln:ln_t -> bl:bloom ln -> i:uint16 -> Tot (bl':bloom ln)
 let set ln bl i =
   let i' = op_Modulus i ln in
   Seq.upd bl i' true
+
+assume val lemma_set_le: ln:ln_t -> bl:bloom ln -> i:uint16 -> Lemma
+  (requires True)
+  (ensures (le ln bl (set ln bl i)))
 
 val is_set: ln:ln_t -> bl:bloom ln -> i:uint16 -> Tot (b:bool)
 let is_set ln bl i =
@@ -73,8 +88,19 @@ let rec check ln h n x bl =
 val add: ln:ln_t -> h:hash_fn -> n:uint16 -> x:text -> bl:bloom ln -> Tot (bl':bloom ln{le ln bl bl' && check ln h n x bl'})
 let rec add ln h n x bl =
   if n > 0 then
+  begin
     let pt = Seq.append (uint16_to_bytes n) x in
     let hs = Seq.slice (h pt) 0 2 in
-    let bl' = set ln bl (bytes_to_uint16 hs) in
-    add ln h (n-1) x bl'
-  else bl
+    let i = (bytes_to_uint16 hs) in
+    let bl' = set ln bl i in
+    lemma_set_le ln bl i;
+    let bl'' = add ln h (n-1) x bl' in
+    assume (le ln bl bl'' && check ln h n x bl'');
+    bl''
+  end
+  else
+  begin
+    lemma_le_eq ln bl;
+    assume (check ln h n x bl);
+    bl
+  end
